uhhhhg.. some progress

src/simpleExamples.v
@@ -225,6 +225,7 @@ Proof.
     unfold my_EQ.
 
     (* wait... this works!*)
+    Check bb0Itree.
     setoid_rewrite bb0Itree.
     unfold denbb0.
     setoid_rewrite bind_ret_l.
@@ -239,11 +240,11 @@ Proof.
     rewrite interp_asm_SetReg.
 
     (* wtf to do with exit *)
-    unfold interp_asm.
-    unfold interp_map.
-    unfold interp_state.
-    (* evaluation to the rescue *)
-    cbn. 
+    (* evaluation to the rescue 
+       we can do this since we provided concrete 
+       register and memory states
+    *)
+    cbn.
     reflexivity.
 Qed.
 (*  This proof is for the no exit version 
@@ -274,68 +275,574 @@ Qed.
     * reflexivity.
 Qed.   
 *) 
-
-
-
-    (* end no exit*)
-
-
-    (* still can't do it.....
-    setoid_rewrite denbb0. *)
-    rewrite bb0ItreeEQ.
-    unfold denbb0.
-    Check bind_ret_l.
-    setoid_rewrite bind_ret_l.
-    setoid_rewrite interp_asm_SetReg.
-    (* dont know what to do with exit*)
-
-    rewrite bb1ItreeEQ.
-    unfold denbb1.
-    Check interp_asm_bind.
-    
-
-    rewrite interp_asm_bind.
-    rewrite interp_asm_bind.
-    setoid_rewrite interp_asm_GetReg.
-
-   setoid_rewrite interp_asm_GetReg.
-
-    Print exit.
-    
-
-
-    unfold exit.
-    rewrite interp_asm_bind.
-    repeat rewrite interp_ret.
-       repeat rewrite interp_state_ret.
-    unfold interp_asm at 2.
-    rewrite interp_vis.
-
-    rewrite interp_asm_bind.
-    rewrite interp_asm_bind.
-    setoid_rewrite interp_asm_ret.
-    
-
-
-    rewrite bb1ItreeEQ.
-    unfold denbb1.
-    
-    rewrite interp_asm_bind.    
-    rewrite interp_asm_bind.
-
-
-    
-    
-    rewrite interp_asm_bind.
-    rewrite interp_asm_bind.
-    setoid_rewrite interp_asm_ret.
-   
-
-    rewrite 
-    simpl.
-    setoid_rewrite interp_asm_SetReg.    
-    
-    
-
-
 End basicdemo.
+
+
+Module deadbranch.
+
+(*
+    transformation where (within a block)
+    if a register is set to 0
+        (track both cases)
+    and then that reg is used for the conditional branch
+    we can convert the conditional branch into a direct jump
+
+*)
+
+(* prove out a simple example *)
+
+(*
+        bb1:
+            r1:= 0
+            Bbrz r1 bb2 bb3
+        /           \ 
+    bb2:        bb3:
+        r2:= 3       r2:= 4
+        Bjmp bb4     Bjmp bb4
+        \           /
+          bb4:
+            r2 := r2 + 1
+            BHault
+
+
+    after dead branch
+
+    bb1:
+        r1 := 0
+        Bjmp bb3
+    bb3:
+        r2 := 4
+        Bjmp bb4
+    bb4:
+        r2 := r2 + 1
+
+    bonus: after block fusion
+
+
+    bb1:
+        r1 := 0
+        r2 := 4
+        r2 := r2 + 1
+
+    bonus: after constant propogation
+        r1 := 0
+        r2 := 4 + 1
+
+    bonus : after constant folding
+
+        r1 := 0
+        r2 := 5
+        
+
+*)
+Check fS f0.
+
+(* definition of the basic blocks *)
+Definition bb1 : block (fin 2):= 
+after [
+    Imov 1 (Oimm 0)
+] (Bbrz 1 f0 (fS f0)).
+
+Definition bb2 : block (fin 1) := 
+after [
+    Imov 2 (Oimm 3)
+] (Bjmp f0).
+
+Definition bb3 : block (fin 1) := 
+after [
+    Imov 2 (Oimm 4)
+] (Bjmp f0).
+
+Definition bb4 : block (fin 1) := 
+after [
+    Iadd 2 2 (Oimm 1)
+] (Bhalt).
+
+(* tying them together as assembly *)
+
+(* block -> asm *)
+Definition a_bb1 : asm 1 2 := raw_asm_block bb1.
+Definition a_bb2 : asm 1 1 := raw_asm_block bb2.
+Definition a_bb3 : asm 1 1 := raw_asm_block bb3.
+Definition a_bb4 : asm 2 1 := raw_asm (fun _ => bb4).
+
+(* use asm combinators to link blocks together *)
+
+
+Definition middle : asm (1 + 1) (1 + 1) 
+    := app_asm a_bb2 a_bb3. (* tensor product *)
+Definition bottom : asm (1 + 1) 1
+    := seq_asm middle a_bb4. (* loop combinator + renaming *)
+Definition prog1 : asm 1 1 
+    := seq_asm a_bb1 bottom. (* loop combinator + renaming *)
+
+(* idk which is easier to work with 
+Definition top : asm 1 (1 + 1)
+    := seq_asm a_bb1 middle.
+Definition bottom : asm 1 1
+    := seq_asm top a_bb4.
+*)
+
+
+(* prog1 defines this assembly program 
+
+        bb1:
+            r1:= 0
+            Bbrz r1 bb2 bb3
+        /           \ 
+    bb2:        bb3:
+        r2:= 3       r2:= 4
+        Bjmp bb4     Bjmp bb4
+        \           /
+          bb4:
+            r2 := r2 + 1
+            BHault
+*)
+(* NOTE: we would need phi nodes here for r2
+    LLVM has phi nodes but asm does not
+
+    however, it is not important in this case 
+    since we are going to remove the branch
+*)
+
+Definition bb1' : block (fin 1) := 
+after [
+    Imov 1 (Oimm 0)
+] (Bjmp f0).
+
+Definition bb3' : block (fin 1) := 
+after [
+    Imov 2 (Oimm 4)
+] (Bjmp f0).
+
+Definition bb4' : block (fin 1) := 
+after [
+    Iadd 2  2 (Oimm 1)
+] (Bhalt).
+
+Definition a_bb1' : asm 1 1 := raw_asm_block bb1'.
+Definition a_bb3' : asm 1 1 := raw_asm_block bb3'.
+Definition a_bb4' : asm 1 1 := raw_asm_block bb4'.
+
+Definition prog2 : asm 1 1 := seq_asm a_bb1' (seq_asm a_bb3' a_bb4').
+
+(* prog2 defines this assembly program
+    bb1':
+        r1 := 0
+        Bjmp bb3'
+    bb3':
+        r2 := 4
+        Bjmp bb4'
+    bb4':
+        r2 := r2 + 1 
+*)
+
+(* to talk about bisimilarity of these programs
+    we need to denote them as itrees
+
+    to do that, we need to determine what effects (E) we are using.
+
+    We will work with an effect E that 
+        HasRegs:
+            Reg  :=
+	            GetReg : reg -> Reg value 
+              | SetReg : reg -> value -> Reg unit.
+
+        HasMemory:
+            Memory := 
+                Load : addr -> Memory value 
+              | Store : addr -> value -> Memory unit.
+
+        HasExit 
+            Exit :=
+                Done : Exit void
+    *)
+Print Exit.
+Context {E' : Type -> Type}.
+Context {HasRegs : Reg -< E'}.
+Context {HasMemory : Memory -< E'}.
+Context {HasExit : Exit -< E'}.
+    
+Definition E := Reg +' Memory +' Exit +' E'.
+
+Notation denote_bk := (denote_bk (E := E)).
+Notation denote_bks := (denote_bks (E := E)).
+Notation denote_asm := (denote_asm (E := E)).
+
+Lemma pointfree (p: asm 1 1)(t :ktree_fin E 1 1) :
+    denote_asm p ⩯ t ->
+    denote_asm p f0 ≈ t f0.
+Admitted.
+
+Lemma pointed (k1 k2 :ktree_fin E 1 1) :
+     k1 f0 ≈ k2 f0 ->
+    k1 ⩯ k2.
+Admitted.
+
+(* now we denote the assembly programs as itrees *)
+(* NOTE: 
+    ktree := (A -> itree E B)
+    is a useful abstraction for reasoning
+*)
+Definition kprog1 : ktree_fin E 1 1 := denote_asm prog1.
+Definition kprog2 : ktree_fin E 1 1 := denote_asm prog2.
+
+Definition iprog1 : itree E (fin 1):= kprog1 f0.
+Definition iprog2 : itree E (fin 1):= kprog2 f0.
+
+
+(* helper lemmas - move these*)
+Lemma seq_asm_correct {A B C} (ab : asm A B) (bc : asm B C) :
+      denote_asm (seq_asm ab bc)
+    ⩯ denote_asm ab >>> denote_asm bc.
+  Proof.
+    unfold seq_asm.
+    rewrite loop_asm_correct, relabel_asm_correct, app_asm_correct.
+    rewrite fmap_id0, cat_id_r, fmap_swap.
+    apply cat_from_loop.
+  Qed.
+
+(* helper lemmas for denoting each basic block *)
+Lemma den_bb1 : denote_asm a_bb1 ⩯
+(fun _ : fin 1 =>
+ (
+    v <- Ret 0;; 
+    trigger (SetReg 1 v));;
+    val <- trigger (GetReg 1);;
+    (if val : nat
+    then Ret f0 
+    else Ret (fS f0))).
+Proof. 
+    unfold a_bb1.
+    setoid_rewrite raw_asm_block_correct_lifted.
+    unfold bb1.
+    reflexivity.
+Qed.
+
+Lemma den_bb1_pt : 
+    denote_asm a_bb1 f0 
+≈
+ (
+    v <- Ret 0;; 
+    trigger (SetReg 1 v));;
+    val <- trigger (GetReg 1);;
+    (if val : nat
+    then Ret f0 
+    else Ret (fS f0)).
+Proof.
+Admitted.
+
+
+Lemma den_bb2 : denote_asm a_bb2 ⩯
+(fun _ : fin 1 => (
+    v <- Ret 3;; 
+    trigger (SetReg 2 v));; 
+    Ret f0).
+Proof.
+    unfold a_bb2.
+    setoid_rewrite raw_asm_block_correct_lifted.
+    unfold bb2.
+    simpl.
+    reflexivity.
+Qed.
+
+Lemma den_bb3 : denote_asm a_bb3 ⩯
+(fun _ : fin 1 => (
+    v <- Ret 4;; 
+    trigger (SetReg 2 v));; 
+    Ret f0).
+Proof.
+    unfold a_bb3.
+    setoid_rewrite raw_asm_block_correct_lifted.
+    unfold bb3.
+    simpl.
+    reflexivity.
+Qed.
+
+Lemma den_bb4 : denote_asm a_bb4 ⩯
+(fun _ : fin 2 => 
+(
+    lv <- trigger (GetReg 2);;
+    rv <- Ret 1;; 
+    trigger (SetReg 2 (lv + rv))
+);; exit).
+Proof.
+    unfold a_bb4.
+    setoid_rewrite raw_asm_correct.
+    unfold bb4.
+    reflexivity.
+Qed.
+
+Lemma den_bb1' : denote_asm a_bb1' ⩯
+(fun _ : fin 1 => (
+    v <- Ret 0;; 
+    trigger (SetReg 1 v));; 
+    Ret f0).
+Proof.
+    unfold a_bb1'.
+    setoid_rewrite raw_asm_block_correct_lifted.
+    unfold bb1'.
+    simpl.
+    reflexivity.
+Qed.
+
+Lemma den_bb3' : denote_asm a_bb3' ⩯
+(fun _ : fin 1 => (
+    v <- Ret 4;; 
+    trigger (SetReg 2 v));; 
+    Ret f0).
+Proof.
+    unfold a_bb3'.
+    setoid_rewrite raw_asm_block_correct_lifted.
+    unfold bb3'.
+    simpl.
+    reflexivity.
+Qed.
+
+Lemma den_bb4' : denote_asm a_bb4' ⩯
+(fun _ : fin 1 => (
+    lv <- trigger (GetReg 2);;
+    rv <- Ret 1;; 
+    trigger (SetReg 2 (lv + rv)))
+    ;; exit).
+Proof.
+    unfold a_bb4'.
+    setoid_rewrite raw_asm_block_correct_lifted.
+    unfold bb4'.
+    simpl.
+    reflexivity.
+Qed.
+
+(*  TODO check this claim 
+    we cannot prove
+        iprog1 ≈ iprog2
+
+    That is because ≈ only says when two programs
+        are syntacticaly similar.
+
+    - explain rel_asm
+    - explain use concrete initial state
+*)
+
+(* make syntax for this *)
+Definition my_EQ (t1 t2 : itree E (fin 1)) : Prop :=
+    (eutt rel_asm)
+        (interp_asm t1 [] [])
+        (interp_asm t2 [] []).
+
+
+
+Definition foo : itree E (fin 1) := Ret f0.
+Definition bar : ktree_fin E 1 1 := fun _ => foo.
+Lemma den_prog1 : 
+    denote_asm prog1 
+⩯ 
+    denote_asm a_bb1 >>>
+    (bimap 
+        (denote_asm a_bb2) 
+        (denote_asm a_bb3) >>>
+    denote_asm a_bb4).
+    unfold prog1.
+
+    setoid_rewrite seq_asm_correct.
+    unfold bottom.
+    setoid_rewrite seq_asm_correct.
+    unfold middle.
+    setoid_rewrite app_asm_correct.
+    reflexivity.
+Qed.
+
+Lemma den_prog1' : 
+    denote_asm prog1 f0
+≈ 
+    (denote_asm a_bb1 >>>
+    (bimap 
+        (denote_asm a_bb2) 
+        (denote_asm a_bb3) >>>
+    denote_asm a_bb4)) f0.
+Proof.
+    apply pointfree.
+    apply den_prog1.
+Qed.
+
+(* (denote_asm a_bb1 >>>
+ (case_ (denote_asm a_bb2 >>> inl_) (denote_asm a_bb3 >>> inr_) >>>
+  denote_asm a_bb4)) f0 ≈ Ret f0*)
+
+Lemma asdfasdf : 
+    (denote_asm a_bb1' >>> denote_asm a_bb3') f0 
+    ≈ 
+    (n <- denote_asm a_bb1' f0 ;; denote_asm a_bb3' n) .
+Admitted.
+
+
+Lemma blarg : (denote_asm prog1 f0) ≈  Ret f0.
+Proof.
+    setoid_rewrite den_prog1'.
+    cbn.
+
+    
+Admitted.
+
+Print my_EQ.
+(* show that the dead branch can be eliminated *)
+Lemma deadbranch : my_EQ iprog1 iprog2.
+Proof.
+    unfold my_EQ.
+    unfold iprog1.
+    unfold kprog1.
+    setoid_rewrite blarg.
+    setoid_rewrite interp_asm_ret.
+    Check interp_asm.
+    Check den_prog1.
+    Check den_prog1'.
+    setoid_rewrite den_prog1'.
+    Check den_bb1.
+
+    setoid_rewrite den_bb1.
+    
+    (interp_asm
+    ((denote_asm a_bb1 >>>
+      (bimap (denote_asm a_bb2) (denote_asm a_bb3) >>>
+       denote_asm a_bb4)) f0) [] [])
+
+
+
+
+(*iprog1 ≈ iprog2 (eutt eq)
+ what is the version for ktrees?
+ what is the difference between ≅ (eq_itree eq)
+                        and ≈ (eutt eq) ?
+
+"Note that the ⩯ notation in the scope of [ktree] desugars to [eutt_ktree],
+      i.e. pointwise [eutt eq]."                        
+*)
+
+Remark cantProve : iprog1 ≈ iprog2.
+ unfold iprog1.
+ unfold kprog1.
+ unfold prog1.
+ Check raw_asm_block_correct_lifted.
+ Check raw_asm_block_correct.
+ rewrite seq_asm_correct_lifted.
+
+Print eq_itree.
+Remark cantProve : kprog1 ⩯ kprog2.
+ unfold kprog1. 
+ unfold prog1. (* use ktrees, stupid binder*)
+
+ (*     rewrite raw_asm_block_correct.
+    normally i'd use this.. 
+    note that it removes the application to "f0"
+
+    How can I get rid of the "f0"?
+*)
+ rewrite seq_asm_correct.
+ 
+ unfold a_bb1.
+ rewrite raw_asm_block_correct_lifted.
+ rewrite denote_bk_corect.
+
+ setoid_rewrite loop_asm_correct.
+(*  we cannot prove
+        iprog1 ≈ iprog2
+
+    That is because ≈ only says when two programs are syntacticaly similar
+
+
+
+
+
+
+
+    Definition rel_asm {B} : memory * (registers * B) -> memory * (registers * B) -> Prop :=
+  prod_rel EQ_memory (prod_rel (EQ_registers 0) eq).
+
+we cannot say that iprog1 and iprog2 are bisimilar *)
+
+(* asm programs denoted as ktrees *)
+
+(* concrete initial state *)
+
+
+Definition my_EQ (t1 t2 : ktree_fin E 1 1) : Prop :=
+    (eutt rel_asm)
+        (interp_asm (t1 f0) initialMemSta(**
+        Definition iprog1_denoted : itree E (fin 1).
+        apply iprog1.
+        *)te initialRegState)
+        (interp_asm (t2 f0) initialMemState initialRegState).
+
+
+
+(* is this going to require renaming labels...?*)
+
+Definition deadbranch_branch {lbl} (b : branch lbl) := 
+    match b with 
+    | Bbrz ()
+
+Definition deadbranch_block {lbl} (bb : block lbl) := 
+    match b with 
+    | bbb
+
+
+End deadbranch.
+
+(* 
+cruft 
+
+(*
+
+
+Remark den_prog1 : iprog1 ≈ bar f0.
+    unfold iprog1.
+    unfold kprog1.
+    apply pointfree.
+
+    unfold prog1.
+
+    setoid_rewrite seq_asm_correct.
+    setoid_rewrite den_bb1.
+
+    unfold bottom.
+    setoid_rewrite seq_asm_correct.
+    setoid_rewrite den_bb4.
+
+    unfold middle.
+    setoid_rewrite app_asm_correct.
+    setoid_rewrite den_bb2.
+    setoid_rewrite den_bb3.
+
+
+    apply pointed.
+    
+    cbn.
+
+
+Admitted.
+
+Check to_bif.
+Definition den_prog1 : itree E (fin 1):= 
+y  <-
+    ((v <- Ret 0;; 
+      trigger (SetReg 1 v));;
+     val <- trigger (GetReg 1);;
+    (if val : nat 
+    then Ret (f0 : fin (1 + 1)) 
+    else Ret ((fS f0): fin (1 + 1)))) : fin (1 + 1);;
+(y0 <- to_bif y;;
+ case_
+   ((fun _ : fin 1 =>
+     (v <- Ret 3;; 
+     trigger (SetReg 2 v));; 
+     Ret f0) >>> inl_)
+   ((fun _ : fin 1 =>
+     (v <- Ret 4;; 
+     trigger (SetReg 2 v));; 
+     Ret f0) >>> inr_)
+   y0);;
+(lv <- trigger (GetReg 2);;
+ rv <- Ret 1;; 
+ trigger (SetReg 2 (lv + rv)))
+ ;; exit.
+*)*)
